beta/syntax.v
@@ -13,7 +13,7 @@ Inductive tm  : Type :=
   | tUniv : ( nat   ) -> tm 
   | tTrue : tm 
   | tFalse : tm 
-  | tIf : ( tm   ) -> ( tm   ) -> ( tm   ) -> tm 
+  | tIf : ( tm   ) -> ( tm   ) -> ( tm   ) -> ( tm   ) -> tm 
   | tBool : tm 
   | tEq : ( tm   ) -> ( tm   ) -> ( tm   ) -> tm 
   | tJ : ( tm   ) -> ( tm   ) -> ( tm   ) -> ( tm   ) -> tm 
@@ -40,7 +40,7 @@ Proof. congruence. Qed.
 Lemma congr_tFalse  : tFalse  = tFalse  .
 Proof. congruence. Qed.
 
-Lemma congr_tIf  { s0 : tm   } { s1 : tm   } { s2 : tm   } { t0 : tm   } { t1 : tm   } { t2 : tm   } (H1 : s0 = t0) (H2 : s1 = t1) (H3 : s2 = t2) : tIf  s0 s1 s2 = tIf  t0 t1 t2 .
+Lemma congr_tIf  { s0 : tm   } { s1 : tm   } { s2 : tm   } { s3 : tm   } { t0 : tm   } { t1 : tm   } { t2 : tm   } { t3 : tm   } (H1 : s0 = t0) (H2 : s1 = t1) (H3 : s2 = t2) (H4 : s3 = t3) : tIf  s0 s1 s2 s3 = tIf  t0 t1 t2 t3 .
 Proof. congruence. Qed.
 
 Lemma congr_tBool  : tBool  = tBool  .
@@ -68,7 +68,7 @@ Fixpoint ren_tm   (xitm : ( fin ) -> fin) (s : tm ) : tm  :=
     | tUniv  s0 => tUniv  ((fun x => x) s0)
     | tTrue   => tTrue 
     | tFalse   => tFalse 
-    | tIf  s0 s1 s2 => tIf  ((ren_tm xitm) s0) ((ren_tm xitm) s1) ((ren_tm xitm) s2)
+    | tIf  s0 s1 s2 s3 => tIf  ((ren_tm (upRen_tm_tm xitm)) s0) ((ren_tm xitm) s1) ((ren_tm xitm) s2) ((ren_tm xitm) s3)
     | tBool   => tBool 
     | tEq  s0 s1 s2 => tEq  ((ren_tm xitm) s0) ((ren_tm xitm) s1) ((ren_tm xitm) s2)
     | tJ  s0 s1 s2 s3 => tJ  ((ren_tm xitm) s0) ((ren_tm xitm) s1) ((ren_tm xitm) s2) ((ren_tm xitm) s3)
@@ -88,7 +88,7 @@ Fixpoint subst_tm   (sigmatm : ( fin ) -> tm ) (s : tm ) : tm  :=
     | tUniv  s0 => tUniv  ((fun x => x) s0)
     | tTrue   => tTrue 
     | tFalse   => tFalse 
-    | tIf  s0 s1 s2 => tIf  ((subst_tm sigmatm) s0) ((subst_tm sigmatm) s1) ((subst_tm sigmatm) s2)
+    | tIf  s0 s1 s2 s3 => tIf  ((subst_tm (up_tm_tm sigmatm)) s0) ((subst_tm sigmatm) s1) ((subst_tm sigmatm) s2) ((subst_tm sigmatm) s3)
     | tBool   => tBool 
     | tEq  s0 s1 s2 => tEq  ((subst_tm sigmatm) s0) ((subst_tm sigmatm) s1) ((subst_tm sigmatm) s2)
     | tJ  s0 s1 s2 s3 => tJ  ((subst_tm sigmatm) s0) ((subst_tm sigmatm) s1) ((subst_tm sigmatm) s2) ((subst_tm sigmatm) s3)
@@ -111,7 +111,7 @@ Fixpoint idSubst_tm  (sigmatm : ( fin ) -> tm ) (Eqtm : forall x, sigmatm x = (v
     | tUniv  s0 => congr_tUniv ((fun x => (eq_refl) x) s0)
     | tTrue   => congr_tTrue 
     | tFalse   => congr_tFalse 
-    | tIf  s0 s1 s2 => congr_tIf ((idSubst_tm sigmatm Eqtm) s0) ((idSubst_tm sigmatm Eqtm) s1) ((idSubst_tm sigmatm Eqtm) s2)
+    | tIf  s0 s1 s2 s3 => congr_tIf ((idSubst_tm (up_tm_tm sigmatm) (upId_tm_tm (_) Eqtm)) s0) ((idSubst_tm sigmatm Eqtm) s1) ((idSubst_tm sigmatm Eqtm) s2) ((idSubst_tm sigmatm Eqtm) s3)
     | tBool   => congr_tBool 
     | tEq  s0 s1 s2 => congr_tEq ((idSubst_tm sigmatm Eqtm) s0) ((idSubst_tm sigmatm Eqtm) s1) ((idSubst_tm sigmatm Eqtm) s2)
     | tJ  s0 s1 s2 s3 => congr_tJ ((idSubst_tm sigmatm Eqtm) s0) ((idSubst_tm sigmatm Eqtm) s1) ((idSubst_tm sigmatm Eqtm) s2) ((idSubst_tm sigmatm Eqtm) s3)
@@ -134,7 +134,7 @@ Fixpoint extRen_tm   (xitm : ( fin ) -> fin) (zetatm : ( fin ) -> fin) (Eqtm : f
     | tUniv  s0 => congr_tUniv ((fun x => (eq_refl) x) s0)
     | tTrue   => congr_tTrue 
     | tFalse   => congr_tFalse 
-    | tIf  s0 s1 s2 => congr_tIf ((extRen_tm xitm zetatm Eqtm) s0) ((extRen_tm xitm zetatm Eqtm) s1) ((extRen_tm xitm zetatm Eqtm) s2)
+    | tIf  s0 s1 s2 s3 => congr_tIf ((extRen_tm (upRen_tm_tm xitm) (upRen_tm_tm zetatm) (upExtRen_tm_tm (_) (_) Eqtm)) s0) ((extRen_tm xitm zetatm Eqtm) s1) ((extRen_tm xitm zetatm Eqtm) s2) ((extRen_tm xitm zetatm Eqtm) s3)
     | tBool   => congr_tBool 
     | tEq  s0 s1 s2 => congr_tEq ((extRen_tm xitm zetatm Eqtm) s0) ((extRen_tm xitm zetatm Eqtm) s1) ((extRen_tm xitm zetatm Eqtm) s2)
     | tJ  s0 s1 s2 s3 => congr_tJ ((extRen_tm xitm zetatm Eqtm) s0) ((extRen_tm xitm zetatm Eqtm) s1) ((extRen_tm xitm zetatm Eqtm) s2) ((extRen_tm xitm zetatm Eqtm) s3)
@@ -157,7 +157,7 @@ Fixpoint ext_tm   (sigmatm : ( fin ) -> tm ) (tautm : ( fin ) -> tm ) (Eqtm : fo
     | tUniv  s0 => congr_tUniv ((fun x => (eq_refl) x) s0)
     | tTrue   => congr_tTrue 
     | tFalse   => congr_tFalse 
-    | tIf  s0 s1 s2 => congr_tIf ((ext_tm sigmatm tautm Eqtm) s0) ((ext_tm sigmatm tautm Eqtm) s1) ((ext_tm sigmatm tautm Eqtm) s2)
+    | tIf  s0 s1 s2 s3 => congr_tIf ((ext_tm (up_tm_tm sigmatm) (up_tm_tm tautm) (upExt_tm_tm (_) (_) Eqtm)) s0) ((ext_tm sigmatm tautm Eqtm) s1) ((ext_tm sigmatm tautm Eqtm) s2) ((ext_tm sigmatm tautm Eqtm) s3)
     | tBool   => congr_tBool 
     | tEq  s0 s1 s2 => congr_tEq ((ext_tm sigmatm tautm Eqtm) s0) ((ext_tm sigmatm tautm Eqtm) s1) ((ext_tm sigmatm tautm Eqtm) s2)
     | tJ  s0 s1 s2 s3 => congr_tJ ((ext_tm sigmatm tautm Eqtm) s0) ((ext_tm sigmatm tautm Eqtm) s1) ((ext_tm sigmatm tautm Eqtm) s2) ((ext_tm sigmatm tautm Eqtm) s3)
@@ -177,7 +177,7 @@ Fixpoint compRenRen_tm    (xitm : ( fin ) -> fin) (zetatm : ( fin ) -> fin) (rho
     | tUniv  s0 => congr_tUniv ((fun x => (eq_refl) x) s0)
     | tTrue   => congr_tTrue 
     | tFalse   => congr_tFalse 
-    | tIf  s0 s1 s2 => congr_tIf ((compRenRen_tm xitm zetatm rhotm Eqtm) s0) ((compRenRen_tm xitm zetatm rhotm Eqtm) s1) ((compRenRen_tm xitm zetatm rhotm Eqtm) s2)
+    | tIf  s0 s1 s2 s3 => congr_tIf ((compRenRen_tm (upRen_tm_tm xitm) (upRen_tm_tm zetatm) (upRen_tm_tm rhotm) (up_ren_ren (_) (_) (_) Eqtm)) s0) ((compRenRen_tm xitm zetatm rhotm Eqtm) s1) ((compRenRen_tm xitm zetatm rhotm Eqtm) s2) ((compRenRen_tm xitm zetatm rhotm Eqtm) s3)
     | tBool   => congr_tBool 
     | tEq  s0 s1 s2 => congr_tEq ((compRenRen_tm xitm zetatm rhotm Eqtm) s0) ((compRenRen_tm xitm zetatm rhotm Eqtm) s1) ((compRenRen_tm xitm zetatm rhotm Eqtm) s2)
     | tJ  s0 s1 s2 s3 => congr_tJ ((compRenRen_tm xitm zetatm rhotm Eqtm) s0) ((compRenRen_tm xitm zetatm rhotm Eqtm) s1) ((compRenRen_tm xitm zetatm rhotm Eqtm) s2) ((compRenRen_tm xitm zetatm rhotm Eqtm) s3)
@@ -200,7 +200,7 @@ Fixpoint compRenSubst_tm    (xitm : ( fin ) -> fin) (tautm : ( fin ) -> tm ) (th
     | tUniv  s0 => congr_tUniv ((fun x => (eq_refl) x) s0)
     | tTrue   => congr_tTrue 
     | tFalse   => congr_tFalse 
-    | tIf  s0 s1 s2 => congr_tIf ((compRenSubst_tm xitm tautm thetatm Eqtm) s0) ((compRenSubst_tm xitm tautm thetatm Eqtm) s1) ((compRenSubst_tm xitm tautm thetatm Eqtm) s2)
+    | tIf  s0 s1 s2 s3 => congr_tIf ((compRenSubst_tm (upRen_tm_tm xitm) (up_tm_tm tautm) (up_tm_tm thetatm) (up_ren_subst_tm_tm (_) (_) (_) Eqtm)) s0) ((compRenSubst_tm xitm tautm thetatm Eqtm) s1) ((compRenSubst_tm xitm tautm thetatm Eqtm) s2) ((compRenSubst_tm xitm tautm thetatm Eqtm) s3)
     | tBool   => congr_tBool 
     | tEq  s0 s1 s2 => congr_tEq ((compRenSubst_tm xitm tautm thetatm Eqtm) s0) ((compRenSubst_tm xitm tautm thetatm Eqtm) s1) ((compRenSubst_tm xitm tautm thetatm Eqtm) s2)
     | tJ  s0 s1 s2 s3 => congr_tJ ((compRenSubst_tm xitm tautm thetatm Eqtm) s0) ((compRenSubst_tm xitm tautm thetatm Eqtm) s1) ((compRenSubst_tm xitm tautm thetatm Eqtm) s2) ((compRenSubst_tm xitm tautm thetatm Eqtm) s3)
@@ -223,7 +223,7 @@ Fixpoint compSubstRen_tm    (sigmatm : ( fin ) -> tm ) (zetatm : ( fin ) -> fin)
     | tUniv  s0 => congr_tUniv ((fun x => (eq_refl) x) s0)
     | tTrue   => congr_tTrue 
     | tFalse   => congr_tFalse 
-    | tIf  s0 s1 s2 => congr_tIf ((compSubstRen_tm sigmatm zetatm thetatm Eqtm) s0) ((compSubstRen_tm sigmatm zetatm thetatm Eqtm) s1) ((compSubstRen_tm sigmatm zetatm thetatm Eqtm) s2)
+    | tIf  s0 s1 s2 s3 => congr_tIf ((compSubstRen_tm (up_tm_tm sigmatm) (upRen_tm_tm zetatm) (up_tm_tm thetatm) (up_subst_ren_tm_tm (_) (_) (_) Eqtm)) s0) ((compSubstRen_tm sigmatm zetatm thetatm Eqtm) s1) ((compSubstRen_tm sigmatm zetatm thetatm Eqtm) s2) ((compSubstRen_tm sigmatm zetatm thetatm Eqtm) s3)
     | tBool   => congr_tBool 
     | tEq  s0 s1 s2 => congr_tEq ((compSubstRen_tm sigmatm zetatm thetatm Eqtm) s0) ((compSubstRen_tm sigmatm zetatm thetatm Eqtm) s1) ((compSubstRen_tm sigmatm zetatm thetatm Eqtm) s2)
     | tJ  s0 s1 s2 s3 => congr_tJ ((compSubstRen_tm sigmatm zetatm thetatm Eqtm) s0) ((compSubstRen_tm sigmatm zetatm thetatm Eqtm) s1) ((compSubstRen_tm sigmatm zetatm thetatm Eqtm) s2) ((compSubstRen_tm sigmatm zetatm thetatm Eqtm) s3)
@@ -246,7 +246,7 @@ Fixpoint compSubstSubst_tm    (sigmatm : ( fin ) -> tm ) (tautm : ( fin ) -> tm 
     | tUniv  s0 => congr_tUniv ((fun x => (eq_refl) x) s0)
     | tTrue   => congr_tTrue 
     | tFalse   => congr_tFalse 
-    | tIf  s0 s1 s2 => congr_tIf ((compSubstSubst_tm sigmatm tautm thetatm Eqtm) s0) ((compSubstSubst_tm sigmatm tautm thetatm Eqtm) s1) ((compSubstSubst_tm sigmatm tautm thetatm Eqtm) s2)
+    | tIf  s0 s1 s2 s3 => congr_tIf ((compSubstSubst_tm (up_tm_tm sigmatm) (up_tm_tm tautm) (up_tm_tm thetatm) (up_subst_subst_tm_tm (_) (_) (_) Eqtm)) s0) ((compSubstSubst_tm sigmatm tautm thetatm Eqtm) s1) ((compSubstSubst_tm sigmatm tautm thetatm Eqtm) s2) ((compSubstSubst_tm sigmatm tautm thetatm Eqtm) s3)
     | tBool   => congr_tBool 
     | tEq  s0 s1 s2 => congr_tEq ((compSubstSubst_tm sigmatm tautm thetatm Eqtm) s0) ((compSubstSubst_tm sigmatm tautm thetatm Eqtm) s1) ((compSubstSubst_tm sigmatm tautm thetatm Eqtm) s2)
     | tJ  s0 s1 s2 s3 => congr_tJ ((compSubstSubst_tm sigmatm tautm thetatm Eqtm) s0) ((compSubstSubst_tm sigmatm tautm thetatm Eqtm) s1) ((compSubstSubst_tm sigmatm tautm thetatm Eqtm) s2) ((compSubstSubst_tm sigmatm tautm thetatm Eqtm) s3)
@@ -269,7 +269,7 @@ Fixpoint rinst_inst_tm   (xitm : ( fin ) -> fin) (sigmatm : ( fin ) -> tm ) (Eqt
     | tUniv  s0 => congr_tUniv ((fun x => (eq_refl) x) s0)
     | tTrue   => congr_tTrue 
     | tFalse   => congr_tFalse 
-    | tIf  s0 s1 s2 => congr_tIf ((rinst_inst_tm xitm sigmatm Eqtm) s0) ((rinst_inst_tm xitm sigmatm Eqtm) s1) ((rinst_inst_tm xitm sigmatm Eqtm) s2)
+    | tIf  s0 s1 s2 s3 => congr_tIf ((rinst_inst_tm (upRen_tm_tm xitm) (up_tm_tm sigmatm) (rinstInst_up_tm_tm (_) (_) Eqtm)) s0) ((rinst_inst_tm xitm sigmatm Eqtm) s1) ((rinst_inst_tm xitm sigmatm Eqtm) s2) ((rinst_inst_tm xitm sigmatm Eqtm) s3)
     | tBool   => congr_tBool 
     | tEq  s0 s1 s2 => congr_tEq ((rinst_inst_tm xitm sigmatm Eqtm) s0) ((rinst_inst_tm xitm sigmatm Eqtm) s1) ((rinst_inst_tm xitm sigmatm Eqtm) s2)
     | tJ  s0 s1 s2 s3 => congr_tJ ((rinst_inst_tm xitm sigmatm Eqtm) s0) ((rinst_inst_tm xitm sigmatm Eqtm) s1) ((rinst_inst_tm xitm sigmatm Eqtm) s2) ((rinst_inst_tm xitm sigmatm Eqtm) s3)
